src/Dafny/examples/fs/block_fs.dfy
@@ -1,0 +1,77 @@
+include "indirect_fs.dfy"
+
+module BlockFs
+{
+  import opened Machine
+  import opened ByteSlice
+  import opened FsKinds
+  import opened JrnlTypes
+  import opened JrnlSpec
+  import opened IndirectPos
+  import opened IndFs
+  import C = Collections
+
+  datatype preInodeData = InodeData(blks: seq<Block>)
+  {
+    static const preZero := InodeData(C.repeat(block0, config.total))
+    static const zero: InodeData := preZero
+
+    predicate Valid()
+    {
+      |blks| == config.total
+    }
+  }
+  type InodeData = x:preInodeData | x.Valid() witness preInodeData.preZero
+
+  function inode_data(ino: Ino, data: imap<Pos, Block>): InodeData
+    requires ino_ok(ino)
+    requires data_dom(data)
+  {
+    var blks := seq(config.total,
+      (n:nat) requires n < config.total => data[Pos.from_flat(ino, n)]);
+    InodeData(blks)
+  }
+
+  class BlockFilesys
+  {
+    ghost var data: map<Ino, InodeData>
+    const ifs: IndFilesys;
+
+
+    function metadata(): map<Ino, uint64>
+      reads ifs
+    {
+      ifs.metadata
+    }
+
+    function Repr(): set<object>
+    {
+      {this} + ifs.Repr()
+    }
+
+    predicate {:opaque} ValidData()
+      reads Repr()
+      requires ifs.ValidQ()
+    {
+      && Fs.ino_dom(data)
+      && forall ino: Ino | ino_ok(ino) :: data[ino] == inode_data(ino, ifs.data)
+    }
+
+    predicate Valid()
+      reads Repr()
+    {
+      && ifs.ValidQ()
+      && ValidData()
+    }
+
+    constructor(d: Disk)
+      ensures Valid()
+      ensures data == map ino: Ino | ino_ok(ino) :: InodeData.zero
+    {
+      this.ifs := new IndFilesys(d);
+      this.data := map ino: Ino | ino_ok(ino) :: InodeData.zero;
+      new;
+      reveal ValidData();
+    }
+  }
+}
